Clean up heapExtendJoin_def

Denotational-HeapExtend.thy
@@ -1,106 +1,61 @@
 theory "Denotational-HeapExtend"
-  imports "Denotational-Common" "HOLCF-Set" "HOLCF-Down-Closed"
+  imports "Denotational-Common" "HOLCF-Set" "HOLCF-Down-Closed" "HOLCF-Fix-Join" "Value-Meet"
 begin
+
+
+instantiation fmap :: (type, pcpo) subpcpo_partition
+begin
+  definition "to_bot x = fmap_bottom (fdom x)"
+  lemma [simp]:"fdom (to_bot x) = fdom x"
+    unfolding to_bot_fmap_def by auto
+
+  lemma to_bot_vimage_cone:"to_bot -` {to_bot x} = {z. fmap_bottom (fdom x) \<sqsubseteq> z}"
+    by (auto simp add:to_bot_fmap_def)
+
+  instance  
+  apply default
+  apply (subst to_bot_vimage_cone)
+  apply (rule subpcpo_cone_above)
+  apply (simp add: to_bot_fmap_def fmap_below_dom)
+  apply (simp add: to_bot_fmap_def)
+  done
+end
+
+
+definition heapExtendJoin_cond'
+  where "heapExtendJoin_cond' h eval \<rho> =
+      ((\<forall> \<rho>'. compatible (fmap_expand \<rho> (fdom \<rho> \<union> fst ` set h)) \<rho>' \<longrightarrow>
+             compatible (fmap_expand \<rho> (fdom \<rho> \<union> fst ` set h)) (fmap_expand (heapToEnv h (\<lambda>e. eval e \<rho>')) (fdom \<rho> \<union> fst ` set h))) \<and>
+       (\<forall> e. e\<in> snd`set h \<longrightarrow> cont (eval e)))"
+
+lemma heapExtendJoin_cond'D:
+  assumes "heapExtendJoin_cond' h eval \<rho>"
+  and   "compatible (fmap_expand \<rho> (fdom \<rho> \<union> fst ` set h)) \<rho>'"
+  shows " compatible (fmap_expand \<rho> (fdom \<rho> \<union> fst ` set h)) (fmap_expand (heapToEnv h (\<lambda>e. eval e \<rho>')) (fdom \<rho> \<union> fst ` set h))"
+  using assms unfolding heapExtendJoin_cond'_def  by metis
+
+lemma heapExtendJoin_cond'I:
+  assumes  "\<And> \<rho>'. compatible (fmap_expand \<rho> (fdom \<rho> \<union> fst ` set h)) \<rho>' \<Longrightarrow>
+                   compatible (fmap_expand \<rho> (fdom \<rho> \<union> fst ` set h)) (fmap_expand (heapToEnv h (\<lambda>e. eval e \<rho>')) (fdom \<rho> \<union> fst ` set h))"
+  and "\<And> e. e \<in> snd ` set h \<Longrightarrow> cont (eval e)"
+  shows "heapExtendJoin_cond' h eval \<rho>"
+  using assms unfolding heapExtendJoin_cond'_def by metis
 
 definition heapExtendJoin :: "Env \<Rightarrow> heap \<Rightarrow> (exp \<Rightarrow> Env \<Rightarrow> Value)  \<Rightarrow> (var, Value) fmap"
   where
   "heapExtendJoin \<rho> h eval =
-    (if (\<forall>e \<in> snd ` set h. cont (eval e)) \<and> compatible_fmap \<rho> (heapToEnv h (\<lambda> e. eval e \<rho>) )
-    then fmap_join \<rho> (fixR (fmap_bottom (fst ` set h)) (\<lambda> \<rho>' . heapToEnv h (\<lambda> e. eval e (fmap_join \<rho> \<rho>'))))
-    else fempty)"
+    (if heapExtendJoin_cond' h eval \<rho>
+    then fix_on (fix_join_compat' (fmap_expand \<rho> (fdom \<rho> \<union> fst ` set h)))
+      (\<lambda> \<rho>'. fmap_expand \<rho> (fdom \<rho> \<union> fst ` set h) \<squnion> fmap_expand (heapToEnv h (\<lambda> e. eval e \<rho>')) (fdom \<rho> \<union> fst ` set h))
+    else (fmap_expand \<rho> (fdom \<rho> \<union> fst ` set h)))"
 
-lemma heapExtendJoin_def2:
-  "heapExtendJoin \<rho> h eval =
-    (if (\<forall>e \<in> snd ` set h. cont (eval e)) \<and> compatible_fmap \<rho> (heapToEnv h (\<lambda> e. eval e \<rho>) )
-    then (fixR (fmap_bottom (fdom \<rho> \<union> fst ` set h)) (\<lambda> \<rho>' . fmap_join \<rho> (heapToEnv h (\<lambda> e. eval e \<rho>'))))
-    else fempty)" (is "_ = (if _ then fixR ?x2 ?F2 else _)")
-proof (cases "(\<forall> e \<in> snd ` set h. cont (eval e)) \<and> compatible_fmap \<rho> (heapToEnv h (\<lambda> e. eval e \<rho>))")
-case True
-  let "fixR ?x1 ?F1" = "fixR (fmap_bottom (fst ` set h)) (\<lambda> \<rho>'. heapToEnv h (\<lambda> e. eval e (fmap_join \<rho> \<rho>')))"
-  show ?thesis
-  proof(induct rule: below_antisym[case_names lt gt])
-  case lt
-    have "fmap_join \<rho> (fixR ?x1 ?F1) \<sqsubseteq> fixR (?F2 ?x2) ?F2"
-      apply (rule parallel_fixR_ind)
-      sorry also
-    have "... = fixR ?x2 ?F2" sorry
-    finally show ?case unfolding heapExtendJoin_def using True by auto
-  next
-  case gt
-    have "fixR ?x2 ?F2  \<sqsubseteq> fmap_join \<rho> (fixR ?x1 ?F1)"
-      sorry
-    thus ?case unfolding heapExtendJoin_def using True by auto
-  qed
-next
-case False
-  thus ?thesis unfolding heapExtendJoin_def apply (subst if_not_P, assumption)+ ..
-qed
+lemma fdom_adm:
+   "adm (\<lambda>\<rho>. P (fdom \<rho>))"
+   by (metis admI chain_fdom(2))
 
-definition heapExtendJoin_cond
-  where "heapExtendJoin_cond h eval \<rho> = ((fdom \<rho> \<inter> fst ` set h) = {})"
-
-consts compatible_with_heap_and_env :: "heap \<Rightarrow> (exp \<Rightarrow> Env \<Rightarrow> Value) \<Rightarrow> Env \<Rightarrow> Env set"
-
-lemma heapExtendJoin_def3:
-  "heapExtendJoin \<rho> h eval =
-    (if heapExtendJoin_cond h eval \<rho>
-    then fix_on (compatible_with_heap_and_env h eval \<rho>) (\<lambda> \<rho>'. fmap_join \<rho> (heapToEnv h (\<lambda> e. eval e \<rho>')))
-    else fempty)"
-sorry
-
-lemma subpcpo_compat_h_e:
-  "subpcpo (compatible_with_heap_and_env h ESem x)" sorry
-
-lemma closed_on_compat_h_e:
-  "closed_on (compatible_with_heap_and_env h ESem x)
-     (\<lambda>\<rho>'. fmap_join x (heapToEnv h (\<lambda>e. ESem e \<rho>')))" sorry
-
-lemma cont_on_compat_h_e:
-  "cont_on (compatible_with_heap_and_env h ESem x)
-     (\<lambda>\<rho>'. fmap_join x (heapToEnv h (\<lambda>e. ESem e \<rho>')))" sorry
-
-lemma compt_h_eD:
-  "\<rho> \<in> compatible_with_heap_and_env h ESem x \<Longrightarrow> compatible_fmap x (heapToEnv h (\<lambda>e. ESem e \<rho>))" sorry
-
-lemma bottom_of_compat_h_e:
-  "bottom_of (compatible_with_heap_and_env h ESem x) = fmap_bottom (fdom x \<union> fst ` set h)" sorry
-
-lemma heapExtendJoin_mono':
-  assumes "\<And> e. e \<in> snd ` set h \<Longrightarrow> cont (ESem e)"
-  shows "monofun (\<lambda>\<rho>. heapExtendJoin \<rho> h ESem)"
-proof (rule monofunI)
-case (goal1 x y)
-  hence [simp]:"fdom y = fdom x"
-    by (metis fmap_below_dom)
-  have subset:
-    "compatible_with_heap_and_env h ESem y \<subseteq> compatible_with_heap_and_env h ESem x" sorry
-  have same_bottom:
-    "bottom_of (compatible_with_heap_and_env h ESem x) = bottom_of (compatible_with_heap_and_env h ESem y)"
-    by (simp add: bottom_of_compat_h_e)
-
-  show ?case
-  proof(cases "fdom x \<inter> (fst ` set h) = {}")
-  case True[simp]
-    show ?thesis
-      unfolding heapExtendJoin_def3
-      unfolding heapExtendJoin_cond_def
-      apply (simp)
-      apply (rule parallel_fix_on_ind[OF subpcpo_compat_h_e subpcpo_compat_h_e _ closed_on_compat_h_e cont_on_compat_h_e  closed_on_compat_h_e cont_on_compat_h_e])
-      apply (rule adm_is_adm_on, simp)
-      apply (subst same_bottom, rule below_refl)
-      apply (drule compt_h_eD)+
-      apply (erule (1) fmap_join_mono[OF _ _ `x \<sqsubseteq> y` ])
-      apply (erule cont2monofunE[OF cont2cont_heapToEnv,rotated ])
-      apply (erule assms(1))
-      done
-  next
-  case False
-    thus ?thesis
-      unfolding heapExtendJoin_def3
-      unfolding heapExtendJoin_cond_def
-      by simp
-  qed
-qed
+lemma fdom_adm_eq[simp]:
+   "adm (\<lambda>\<rho>. fdom \<rho> = z)"
+   by (rule fdom_adm)
 
 (* More special version first, just to check proof *)
 lemma fix_join_cont':
@@ -141,93 +96,401 @@ lemma fix_join_cont':
   apply fact
   done
 
-lemma "compatible_fmap a b \<Longrightarrow> compatible a b"
-  unfolding compatible_def
-  apply (rule exI[where x = "fmap_join a b"] )
-  apply (rule is_lubI)
-  apply (rule is_ubI)
-  apply auto
-  oops
+lemma "fdom \<rho> \<inter> fst ` set h = {} \<Longrightarrow> compatible_fmap \<rho> (heapToEnv h (\<lambda> e. ESem e \<rho>'))"
+  by (rule compatible_fmap_disjoint_fdom, simp)
 
-lemma heapExtendJoin_cont':
-  assumes "\<And> e. e \<in> snd ` set h \<Longrightarrow> cont (ESem e)"
-  shows "cont (\<lambda>\<rho>. heapExtendJoin \<rho> h ESem)"
-proof (rule contI2)
-case goal1 show ?case using assms by (metis heapExtendJoin_mono') 
+lemma compatible_fmap_is_compatible: "compatible_fmap m1 m2 \<Longrightarrow> fdom m1 = fdom m2 \<Longrightarrow> compatible m1 m2"
+  apply (rule compatibleI[of _ "fmap_join m1 m2"])
+  apply (erule (1) fmap_join_below1)
+  apply (erule (1) fmap_join_below2)
+  apply (erule (3) fmap_join_least)
+  done
+
+lemma compatible_is_compatible_fmap: assumes "compatible m1 m2" shows "compatible_fmap m1 m2"
+proof (rule compatible_fmapI, rule compatibleI)
+case (goal1 x)
+  show "the (lookup m1 x) \<sqsubseteq> the (lookup (m1 \<squnion> m2) x)"
+    by (rule fmap_belowE[OF join_above1[OF assms]])
 next
-case (goal2 Y)
-  hence [simp]:"\<And> i. fdom (Y i) = fdom (\<Squnion> i. Y i)" (is "\<And> _ .(_ = ?d)") by (metis chain_fdom)
-
-  show ?case
-  proof(cases "?d \<inter> (fst ` set h) = {}")
-  case True[simp]
-    (* Approach by finding compatible pcpo's: *)
-
-    have "fix_on (compatible_with_heap_and_env h ESem (Lub Y)) (\<lambda>\<rho>'. fmap_join (Lub Y) (heapToEnv h (\<lambda>e. ESem e \<rho>'))) \<sqsubseteq>
-      (\<Squnion> i. fix_on (compatible_with_heap_and_env h ESem (Lub Y)) (\<lambda>\<rho>'. fmap_join (Y i) (heapToEnv h (\<lambda>e. ESem e \<rho>'))))"
-      apply (rule fix_on_cont''[OF `chain Y` subpcpo_compat_h_e])
-      sorry
-
-    show ?thesis
-      unfolding heapExtendJoin_def3
-      unfolding heapExtendJoin_cond_def
-      apply (simp)
-      apply (rule fix_on_cont'[OF `chain Y` subpcpo_compat_h_e closed_on_compat_h_e cont_on_compat_h_e])
-      defer
-      apply (simp add: bottom_of_compat_h_e)
-      sorry
-  next
-  case False
-    thus ?thesis
-      unfolding heapExtendJoin_def3
-      unfolding heapExtendJoin_cond_def
-      by simp
-  qed
+case (goal2 x)
+  show "the (lookup m2 x) \<sqsubseteq> the (lookup (m1 \<squnion> m2) x)"
+    by (rule fmap_belowE[OF join_above2[OF assms]])
+next
+case (goal3 x a)
+  have "m1 \<sqsubseteq> fmap_upd (m1 \<squnion> m2) x a"
+    apply (rule fmap_belowI')
+    apply (simp)[1]
+    apply (metis "HOLCF-Join.join_above1" assms fmap_below_dom goal3(1) insert_absorb)
+    apply (case_tac "xa = x")
+    apply (auto simp add: goal3)
+    by (rule fmap_belowE[OF join_above1[OF assms]])
+  moreover
+  have "m2 \<sqsubseteq> fmap_upd (m1 \<squnion> m2) x a"
+    apply (rule fmap_belowI')
+    apply (simp)[1]
+    apply (metis "HOLCF-Join.join_above2" assms below_fmap_def goal3(2) insert_absorb)
+    apply (case_tac "xa = x")
+    apply (auto simp add: goal3)
+    by (rule fmap_belowE[OF join_above2[OF assms]])
+  ultimately
+  have "m1 \<squnion> m2 \<sqsubseteq> fmap_upd (m1 \<squnion> m2) x a"
+    by (rule join_below[OF assms])
+  moreover
+  have "the (lookup (fmap_upd (m1 \<squnion> m2) x a) x) = a" by simp
+  ultimately  
+  show "the (lookup (m1 \<squnion> m2) x) \<sqsubseteq> a" by (metis fmap_belowE)
 qed
+
+lemma fdom_compatible[simp]:
+  "compatible m1 (m2::('a, 'b::pcpo) fmap) \<Longrightarrow> fdom m1 = fdom m2"
+by (metis join_above1 join_above2 fmap_below_dom)
+
+lemma fdom_join[simp]:
+  "compatible m1 (m2::('a, 'b::pcpo) fmap) \<Longrightarrow> fdom (m1 \<squnion> m2) = fdom m1"
+  by (metis join_above1 fmap_below_dom)
+
+lemma join_is_fmap_join:
+  assumes "compatible m1 (m2::('a, 'b::pcpo) fmap)"
+  shows "m1 \<squnion> m2 = fmap_join m1 m2"
+  apply (rule is_joinI)
+  apply (rule fmap_join_below1[OF compatible_is_compatible_fmap[OF assms] fdom_compatible[OF assms]])
+  apply (rule fmap_join_below2[OF compatible_is_compatible_fmap[OF assms] fdom_compatible[OF assms]])
+  apply (erule (1) fmap_join_least[OF compatible_is_compatible_fmap[OF assms] fdom_compatible[OF assms]])
+  done
+
+lemma the_lookup_compatible:
+  assumes "compatible m1 (m2::('a, 'b::pcpo) fmap)"
+  shows "compatible (the (lookup m1 x)) (the (lookup m2 x))"
+proof(cases "x \<in> fdom m1")
+case True hence "x \<in> fdom m2" by (metis fdom_compatible[OF assms])
+  thus ?thesis
+    by (metis Int_iff True compatible_fmap_def' compatible_is_compatible_fmap[OF assms])
+next
+case False
+  thus ?thesis
+    by (metis assms compatible_refl fdomIff fdom_compatible)
+qed
+
+lemma the_lookup_join:
+  assumes "compatible m1 (m2::('a, 'b::pcpo) fmap)"
+  shows "the (lookup (m1 \<squnion> m2) x) = the (lookup m1 x) \<squnion> the (lookup m2 x)"
+proof(cases "x \<in> fdom m1")
+case True hence "x \<in> fdom m2" by (metis fdom_compatible[OF assms])
+  show ?thesis
+  apply (subst join_is_fmap_join[OF assms])
+  apply (rule lookup_fmap_join1[OF compatible_is_compatible_fmap[OF assms]])
+  by fact+
+next
+case False
+  thus ?thesis by (metis fdomIff join_self fdom_compatible[OF assms] fdom_join[OF assms])
+qed
+
+
+lemma compatible_expand: "compatible_fmap m1 m2 \<Longrightarrow> compatible (fmap_expand m1 (fdom m1 \<union> fdom m2)) (fmap_expand m2 (fdom m1 \<union> fdom m2))"
+  apply (rule compatible_fmap_is_compatible)
+  apply (erule compatible_fmap_expand)
+  apply simp
+  done
+
+lemma fmap_join_expand: "compatible_fmap m1 m2 \<Longrightarrow> fmap_join m1 m2 = (fmap_join (fmap_expand m1 (fdom m1 \<union> fdom m2)) (fmap_expand m2 (fdom m1 \<union> fdom m2)))"
+  apply (rule fmap_eqI)
+  apply simp
+  apply simp
+  apply (erule disjE)
+  apply (case_tac "x \<in> fdom m2")
+  apply (simp add: compatible_is_compatible_fmap[OF compatible_expand])
+  apply (simp add: compatible_is_compatible_fmap[OF compatible_expand])
+  apply (case_tac "x \<in> fdom m1")
+  apply (simp add: compatible_is_compatible_fmap[OF compatible_expand])
+  apply (simp add: compatible_is_compatible_fmap[OF compatible_expand])
+  done
+
+lemma fmap_join_is_join_expand:
+  "compatible_fmap m1 (m2::('a, 'b::pcpo) fmap) \<Longrightarrow> fmap_join m1 m2 = fmap_expand m1 (fdom m1 \<union> fdom m2) \<squnion> fmap_expand m2 (fdom m1 \<union> fdom m2)"
+  apply (subst fmap_join_expand, assumption)
+  apply (erule join_is_fmap_join[symmetric, OF compatible_expand])
+  done
+
+lemma disjoint_is_heapExtendJoin_cond':
+  "fdom \<rho> \<inter> fst ` set h = {} \<Longrightarrow> (\<forall> e \<in> snd`set h.  cont (ESem e)) \<Longrightarrow> heapExtendJoin_cond' h ESem \<rho>"
+  apply (rule heapExtendJoin_cond'I)
+  by (metis compatible_expand compatible_fmap_disjoint_fdom heapToEnv_fdom, metis)
+
+lemma heapExtendJoin_cond'_cont:
+  " heapExtendJoin_cond' h eval \<rho> \<Longrightarrow> cont (\<lambda>x. fmap_expand (heapToEnv h (\<lambda>e. eval e x)) (fdom \<rho> \<union> fst ` set h))"
+unfolding heapExtendJoin_cond'_def
+  apply (rule cont_compose[OF fmap_expand_cont])
+  apply (rule cont2cont_heapToEnv)
+  apply simp
+  done
+
+lemma heapExtendJoin_ind:
+  assumes "heapExtendJoin_cond' h eval \<rho> \<Longrightarrow> subpcpo_syn.adm_on (fix_join_compat' (fmap_expand \<rho> (fdom \<rho> \<union> fst ` set h))) P"
+  assumes "heapExtendJoin_cond' h eval \<rho> \<Longrightarrow> P (to_bot (fmap_expand \<rho> (fdom \<rho> \<union> fst ` set h)))"
+  assumes "\<And> y. heapExtendJoin_cond' h eval \<rho> \<Longrightarrow>
+        y \<in> fix_join_compat' (fmap_expand \<rho> (fdom \<rho> \<union> fst ` set h)) \<Longrightarrow>
+        P y \<Longrightarrow>
+        P (fmap_expand \<rho> (fdom \<rho> \<union> fst ` set h) \<squnion> fmap_expand (heapToEnv h (\<lambda>e. eval e y)) (fdom \<rho> \<union> fst ` set h))"
+  assumes "P (fmap_expand \<rho> (fdom \<rho> \<union> fst ` set h))"
+  shows "P (heapExtendJoin \<rho> h eval)"
+  unfolding heapExtendJoin_def
+  apply (cases "heapExtendJoin_cond' h eval \<rho>")
+  apply (simp)
+  apply (rule fix_on_jfc'_ind)
+  apply (erule heapExtendJoin_cond'_cont)
+  apply (erule (1) heapExtendJoin_cond'D)
+  apply fact+
+  apply (simp)
+  apply (rule assms(4))
+  done
+
+lemma heapExtendJoin_eq:
+  assumes "heapExtendJoin_cond' h eval \<rho>"
+  shows "heapExtendJoin \<rho> h eval = fmap_expand \<rho> (fdom \<rho> \<union> fst ` set h) \<squnion> fmap_expand (heapToEnv h (\<lambda>e. eval e (heapExtendJoin \<rho> h eval))) (fdom \<rho> \<union> fst ` set h)"
+  unfolding heapExtendJoin_def
+  using assms
+  apply (simp)
+  apply (rule fix_on_jfc'_eq)
+  apply (erule heapExtendJoin_cond'_cont)
+  apply (erule (1) heapExtendJoin_cond'D)
+  done
+
+lemma compatible_fmap_bottom[simp]:
+  "fdom x = y \<Longrightarrow> compatible x (fmap_bottom y)"
+  by (metis below.r_refl compatibleI to_bot_fmap_def to_bot_minimal)
+
+lemma heapExtendJoin_compatible[simp]:
+  "compatible (fmap_expand \<rho> (fdom \<rho> \<union> fst ` set \<Gamma>)) (heapExtendJoin \<rho> \<Gamma> ESem)"
+  apply (rule heapExtendJoin_ind)
+  apply (rule adm_is_adm_on)
+  apply (rule compatible_adm2)
+  apply (subst to_bot_fmap_def)
+  apply simp
+  apply (erule (1) compatible_above1[OF heapExtendJoin_cond'D])
+  apply (rule compatible_refl)
+  done  
+
+
+lemma fdom_heapExtendJoin[simp]:
+  "fdom (heapExtendJoin \<rho> h eval) = fdom \<rho> \<union> fst ` set h"
+  apply (rule heapExtendJoin_ind)
+  apply (rule adm_is_adm_on)
+  apply simp
+  apply simp
+  apply (subst fdom_join)
+  apply (erule heapExtendJoin_cond'D)
+  apply simp_all
+  done
+
+lemma lub_eq_range_is_lub:
+  "(\<And> i. F (Y i) \<sqsubseteq> F (Y (Suc i))) \<Longrightarrow> F (\<Squnion> i. Y i) = (\<Squnion> i. F (Y i)) \<Longrightarrow> range (\<lambda>i. F (Y i)::'b::cpo) <<| F (\<Squnion> i. Y i)"
+  apply (erule ssubst)
+  apply (rule cpo_lubI)
+  apply (erule chainI)
+  done
+
+lemma range_is_lubI2:
+  assumes "(\<And> i. F (Y i) \<sqsubseteq> F (Y (Suc i)))"
+  assumes "(\<And> i. F (Y i) \<sqsubseteq> F (\<Squnion>i . Y i))"
+  assumes "F (\<Squnion> i. Y i) \<sqsubseteq> (\<Squnion> i. F (Y i))"
+  shows "range (\<lambda>i. F (Y i)::'b::cpo) <<| F (\<Squnion> i. Y i)"
+proof-
+  have "chain (\<lambda>i. F (Y i))" using assms(1) by (rule chainI)
+  have "(\<Squnion> i. F (Y i)) \<sqsubseteq> F (\<Squnion> i. Y i)" by (rule lub_below[OF `chain _` assms(2)])
+  hence "F (\<Squnion> i. Y i) = (\<Squnion> i. F (Y i))" using assms(3) by (rule below_antisym[rotated])
+  thus ?thesis
+    apply (rule ssubst)
+    apply (rule cpo_lubI[OF `chain _`])
+    done
+qed
+
+lemma heapExtendJoin_monofun'':
+  assumes cont: "\<And> e. e \<in> snd ` set h \<Longrightarrow> cont (ESem e)"
+  assumes cond1: "heapExtendJoin_cond' h ESem \<rho>"
+  assumes cond2: "heapExtendJoin_cond' h ESem \<rho>'"
+  assumes "\<rho> \<sqsubseteq> \<rho>'"
+  shows "heapExtendJoin \<rho> h ESem \<sqsubseteq> heapExtendJoin \<rho>' h ESem"
+    unfolding heapExtendJoin_def
+    unfolding if_P[OF cond1] if_P[OF cond2]
+    apply (simp only: fmap_below_dom[OF `\<rho> \<sqsubseteq> \<rho>'`, symmetric])
+    apply (rule fix_on_jfc'_mono'')
+    apply (rule monofunE[OF fmap_expand_monofun assms(4)])
+    apply (intro cont_compose[OF fmap_expand_cont] cont2cont_heapToEnv assms) apply assumption
+    apply (erule heapExtendJoin_cond'D[OF cond1])
+    apply (erule heapExtendJoin_cond'D[OF cond2, unfolded fmap_below_dom[OF `\<rho> \<sqsubseteq> \<rho>'`, symmetric]])
+    done
 
 
 lemma heapExtendJoin_cont'':
-  "\<lbrakk> (\<And> e. e \<in> snd ` set h \<Longrightarrow> cont (ESem e));
-    fdom (Y 0) \<inter> (fst ` set h) = {} \<rbrakk>
-  \<Longrightarrow> range (\<lambda>i. heapExtendJoin (Y i) h ESem) <<| heapExtendJoin (\<Squnion> i. Y i) h ESem"
-sorry
+  assumes cont: "\<And> e. e \<in> snd ` set h \<Longrightarrow> cont (ESem e)"
+  assumes cond1: "heapExtendJoin_cond' h ESem (\<Squnion> i. Y i)"
+  assumes cond2: "\<And>i. heapExtendJoin_cond' h ESem (Y i)"
+  assumes "chain Y"
+  shows "heapExtendJoin (\<Squnion> i. Y  i) h ESem \<sqsubseteq> (\<Squnion> i. heapExtendJoin (Y i) h ESem)"
+proof-
+  have fdoms[simp]:"\<And> i. fdom (Y i) = fdom (\<Squnion> i. Y i)" (is "\<And> _ .(_ = ?d)") by (metis chain_fdom `chain Y`) 
 
+  have compat_preserve:
+    "\<And> i \<rho>'. compatible (fmap_expand (Y i) (?d \<union> fst ` set h)) \<rho>' \<Longrightarrow>
+            compatible (fmap_expand (Y i) (?d \<union> fst ` set h)) (fmap_expand (heapToEnv h (\<lambda>e. ESem e \<rho>')) (?d \<union> fst ` set h)) "
+     using heapExtendJoin_cond'D[OF cond2] by simp
+
+  have "fix_on       (fix_join_compat' (\<Squnion> i. fmap_expand (Y i)  (?d \<union> fst ` set h)))
+             (\<lambda>\<rho>'.                     (\<Squnion> i. fmap_expand (Y i)  (?d \<union> fst ` set h)) \<squnion>
+                      fmap_expand (heapToEnv h (\<lambda>e. ESem e \<rho>')) (?d \<union> fst ` set h)) \<sqsubseteq>
+       (\<Squnion> i. fix_on  (fix_join_compat'       (fmap_expand (Y i) (?d \<union> fst ` set h)))
+                                        (\<lambda>\<rho>'. fmap_expand (Y i) (?d \<union> fst ` set h) \<squnion>
+                      fmap_expand (heapToEnv h (\<lambda>e. ESem e \<rho>')) (?d \<union> fst ` set h))) "
+    apply (rule fix_on_join_cont'')
+    apply (rule ch2ch_cont[OF fmap_expand_cont `chain Y`])
+    apply (intro cont_compose[OF fmap_expand_cont] cont2cont_heapToEnv assms) apply assumption
+    apply (erule compat_preserve)
+    done
+  thus ?thesis
+    unfolding heapExtendJoin_def
+    unfolding if_P[OF cond1] if_P[OF cond2]
+    by (simp  add: cont2contlubE[OF fmap_expand_cont `chain Y`])
+qed
+
+
+lemma heapExtendJoin_cond'_eqvt[eqvt]:
+ assumes "heapExtendJoin_cond' h eval \<rho>"
+ shows "heapExtendJoin_cond' (\<pi> \<bullet> h) (\<pi> \<bullet> eval) (\<pi> \<bullet> \<rho>)"
+proof (rule heapExtendJoin_cond'I)
+  fix \<rho>'
+  assume "compatible (fmap_expand (\<pi> \<bullet> \<rho>) (fdom (\<pi> \<bullet> \<rho>) \<union> fst ` set (\<pi> \<bullet> h))) \<rho>'"
+  hence "compatible (-\<pi> \<bullet> (fmap_expand (\<pi> \<bullet> \<rho>) (fdom (\<pi> \<bullet> \<rho>) \<union> fst ` set (\<pi> \<bullet> h)))) (-\<pi> \<bullet>\<rho>')"
+    by (rule compatible_eqvt)
+  hence "compatible (fmap_expand \<rho> (fdom \<rho> \<union> fst ` set h)) (-\<pi> \<bullet> \<rho>')"
+    apply perm_simp by (metis pemute_minus_self permute_minus_cancel(1))
+  hence "compatible (fmap_expand \<rho> (fdom \<rho> \<union> fst ` set h))
+           (fmap_expand (heapToEnv h (\<lambda>e. eval e (- \<pi> \<bullet> \<rho>'))) (fdom \<rho> \<union> fst ` set h))"
+    by (rule heapExtendJoin_cond'D[OF assms])
+  hence "compatible (\<pi> \<bullet> (fmap_expand \<rho> (fdom \<rho> \<union> fst ` set h)))
+           (\<pi> \<bullet> (fmap_expand (heapToEnv h (\<lambda>e. eval e (- \<pi> \<bullet> \<rho>'))) (fdom \<rho> \<union> fst ` set h)))"
+    by (rule compatible_eqvt)
+  thus  "compatible (fmap_expand (\<pi> \<bullet> \<rho>) (fdom (\<pi> \<bullet> \<rho>) \<union> fst ` set (\<pi> \<bullet> h)))
+          (fmap_expand (heapToEnv (\<pi> \<bullet> h) (\<lambda>e. (\<pi> \<bullet> eval) e \<rho>')) (fdom (\<pi> \<bullet> \<rho>) \<union> fst ` set (\<pi> \<bullet> h)))"
+    apply (perm_simp)  by (metis (no_types) permute_minus_cancel(2) permute_self)
+next
+  fix e
+  assume "e \<in> snd ` set (\<pi> \<bullet> h)"
+  hence "- \<pi> \<bullet> e \<in> -\<pi> \<bullet> (snd ` set (\<pi> \<bullet> h))" by (metis mem_permute_iff)
+  hence "-\<pi> \<bullet> e \<in> snd ` set h" apply perm_simp by (metis eqvt_bound permute_self unpermute_def)
+  hence "cont (eval (-\<pi> \<bullet> e))" using assms unfolding  heapExtendJoin_cond'_def by metis
+  thus "cont ((\<pi> \<bullet> eval) e)" by (metis perm_still_cont permute_fun_def)
+qed
+
+lemma fix_join_compat'_eqvt[eqvt]:
+  "\<pi> \<bullet> fix_join_compat' (\<rho>::'a::{Bounded_Nonempty_Meet_cpo,subpcpo_partition,cont_pt}) = fix_join_compat' (\<pi> \<bullet> \<rho>)"
+unfolding fix_join_compat'_def
+  by (perm_simp, rule)
+
+
+lemma subcpo_eqvt[eqvt]:
+  fixes S :: "('a::cont_pt) set"
+  assumes "subcpo S"
+  shows "subcpo (\<pi> \<bullet> S)"
+proof(rule subcpoI)
+  fix Y :: "nat \<Rightarrow> 'a"
+  assume "chain Y"
+    hence "chain (-\<pi> \<bullet> Y)" by (rule chain_eqvt)
+  moreover
+  assume "\<And> i. Y i \<in> \<pi> \<bullet> S"
+  hence "\<And> i. - \<pi> \<bullet> Y i \<in> S" by (metis (full_types) mem_permute_iff permute_minus_cancel(1))
+  hence "\<And> i. (- \<pi> \<bullet> Y) i \<in> S" by (metis eqvt_apply permute_pure)
+  ultimately
+  have "(\<Squnion> i. (- \<pi> \<bullet> Y) i) \<in> S" by (metis subcpo.cpo'[OF assms])
+  hence "\<pi> \<bullet> (\<Squnion> i. (- \<pi> \<bullet> Y) i) \<in> \<pi> \<bullet> S"  by (metis mem_permute_iff)
+  find_theorems permute cont
+  thus "(\<Squnion> i. Y i) \<in> \<pi> \<bullet> S"
+    apply -
+    apply (subst (asm) cont2contlubE[OF perm_cont `chain (-\<pi> \<bullet> Y)`])
+    by (metis image_image permute_minus_cancel(1) permute_set_eq_image range_eqvt)
+qed
+
+lemma subpcpo_bot_eqvt[eqvt]:
+  fixes S :: "('a::cont_pt) set"
+  assumes "subpcpo_bot S b"
+  shows "subpcpo_bot (\<pi> \<bullet> S) (\<pi> \<bullet> b)"
+  apply (rule subpcpo_botI)
+  apply (metis subcpo.cpo'[OF subcpo_eqvt[OF subpcpo_is_subcpo[OF subpcpo_bot_is_subpcpo[OF assms]]]])
+  apply (metis bottom_of_subpcpo_bot_there[OF assms] mem_permute_iff)
+  apply (metis (full_types) bottom_of_subpcpo_bot_minimal[OF assms] eqvt_bound mem_permute_iff perm_cont_simp)
+  done
+
+lemma subpcpo_eqvt[eqvt]:
+  fixes S :: "('a::cont_pt) set"
+  assumes "subpcpo S"
+  shows "subpcpo (\<pi> \<bullet> S)"
+  by (rule subpcpo_bot_is_subpcpo[OF subpcpo_bot_eqvt[OF subpcpo_is_subpcpo_bot[OF assms]]])
+
+lemma bottom_of_eqvt:
+  assumes "subpcpo S"
+  shows "\<pi> \<bullet> (bottom_of (S ::('a::cont_pt) set)) = bottom_of (\<pi> \<bullet> S)"
+  by (rule bottom_of_subpcpo_bot[symmetric, OF subpcpo_bot_eqvt[OF  subpcpo_is_subpcpo_bot[OF assms]]])
 
 lemma heapExtendJoin_eqvt[eqvt]:
   "\<pi> \<bullet> heapExtendJoin \<rho> h eval = heapExtendJoin (\<pi> \<bullet> \<rho>) (\<pi> \<bullet> h) (\<pi> \<bullet> eval)"
-proof (cases "(\<forall> e \<in> snd ` set h. cont (eval e)) \<and> compatible_fmap \<rho> (heapToEnv h (\<lambda> e. eval e \<rho>))")
+proof (cases "heapExtendJoin_cond' h eval \<rho>")
   case True
-  moreover hence "(\<forall> e \<in> snd ` set (\<pi> \<bullet> h). cont ((\<pi> \<bullet> eval) e)) \<and> compatible_fmap (\<pi> \<bullet> \<rho>) (heapToEnv (\<pi> \<bullet> h) (\<lambda> e. (\<pi> \<bullet> eval) e (\<pi> \<bullet> \<rho>))) " sorry
-  ultimately show ?thesis
+  hence True_permuted: "heapExtendJoin_cond' (\<pi> \<bullet> h) (\<pi> \<bullet> eval) (\<pi> \<bullet> \<rho>)"
+    by (rule heapExtendJoin_cond'_eqvt)
+
+  have  cont: "cont (\<lambda>x. fmap_expand (heapToEnv h (\<lambda>e. eval e x)) (fdom \<rho> \<union> fst ` set h))"
+   apply (rule cont_compose[OF fmap_expand_cont])
+   apply (rule cont2cont_heapToEnv)
+   using True unfolding heapExtendJoin_cond'_def apply metis
+   done
+
+  have  cont_permuted: "cont (\<lambda>x. fmap_expand (heapToEnv (\<pi> \<bullet> h) (\<lambda>e. (\<pi> \<bullet> eval) e x)) (fdom (\<pi> \<bullet> \<rho>) \<union> fst ` set (\<pi> \<bullet> h)))"
+   apply (rule cont_compose[OF fmap_expand_cont])
+   apply (rule cont2cont_heapToEnv)
+   using True_permuted unfolding heapExtendJoin_cond'_def apply metis
+   done
+
+  show ?thesis
    unfolding heapExtendJoin_def
-   apply -
-   apply (subst if_P, assumption)+
-   apply (subst fmap_join_eqvt)
-   apply (subst fixR_eqvt)
-   apply (auto simp add: fmap_bottom_eqvt)[1]
+   apply (simp only: if_P[OF True] if_P[OF True_permuted])
+   apply (rule parallel_fix_on_ind[OF
+        subpcpo_jfc'
+        subpcpo_jfc'
+        adm_is_adm_on
+        closed_onI[OF closed_jfc'[OF cont heapExtendJoin_cond'D[OF True]]]
+        cont_on_jfc'[OF cont heapExtendJoin_cond'D[OF True]]
+        closed_onI[OF closed_jfc'[OF cont_permuted heapExtendJoin_cond'D[OF True_permuted]]]
+        cont_on_jfc'[OF cont_permuted heapExtendJoin_cond'D[OF True_permuted]]
+        ])
+   apply simp
+   apply assumption+
+   apply (subst bottom_of_eqvt[OF  subpcpo_jfc'])
+   apply (perm_simp, rule)
+   apply perm_simp
+   apply simp
+   done
+next
+case False 
+  hence False_permuted: "\<not> heapExtendJoin_cond' (\<pi> \<bullet> h) (\<pi> \<bullet> eval) (\<pi> \<bullet> \<rho>)"
+    by (metis heapExtendJoin_cond'_eqvt permute_minus_cancel(2))
+  show ?thesis
+   unfolding heapExtendJoin_def
+   apply (simp only: if_not_P[OF False] if_not_P[OF False_permuted])
    apply perm_simp
    apply rule
    done
-next
-case False thus ?thesis
-   unfolding heapExtendJoin_def
-   apply (subst if_not_P, assumption)
-   apply (subst if_not_P)
-   apply  (rule notI)
-   apply  (erule notE)
-   apply  rule
-   apply  (metis perm_still_cont4)
-   apply  (erule conjE)
-   apply  (drule compatible_fmap_eqvt[of _ _ "- \<pi>"])
-   apply  (simp add: permute_fun_def heapToEnv_eqvt)
-   apply (rule fempty_eqvt)
-   done
 qed
 
+
+lemma heapExtendJoin_cond'_cong[fundef_cong]:
+  "\<lbrakk> env1 = env2 ; heap1 = heap2 ; (\<And> e. e \<in> snd ` set heap2 \<Longrightarrow> eval1 e = eval2 e) \<rbrakk>
+      \<Longrightarrow>  heapExtendJoin_cond' heap1 eval1 env1 \<longleftrightarrow> heapExtendJoin_cond'  heap2 eval2 env2"
+  unfolding heapExtendJoin_cond'_def by (auto cong:heapToEnv_cong)
+
 lemma heapExtendJoin_cong[fundef_cong]:
-  "\<lbrakk> env1 = env2 ; heap1 = heap2 ;  (\<And> e. e \<in> snd ` set heap2 \<Longrightarrow> eval1 e = eval2 e) \<rbrakk>
+  "\<lbrakk> env1 = env2 ; heap1 = heap2 ; (\<And> e. e \<in> snd ` set heap2 \<Longrightarrow> eval1 e = eval2 e) \<rbrakk>
       \<Longrightarrow> heapExtendJoin env1 heap1 eval1 = heapExtendJoin env2 heap2 eval2"
   unfolding heapExtendJoin_def
+  unfolding heapExtendJoin_cond'_def
   by (auto cong:heapToEnv_cong)
 
 definition heapExtend :: "Env \<Rightarrow> heap \<Rightarrow> (exp \<Rightarrow> Env \<Rightarrow> Value)  \<Rightarrow> (var, Value) fmap"
